Cleaned some definitions

ntor/Metareduction.ec
@@ -6,7 +6,7 @@ require (*  *) DiffieHellman.
 
 (* ------------------------------------------------------------------------------------------ *)
 (* Introduce stop in original game *)
-module GAKEb_st (S: Server) (C: Client) (H : GAKEc.HROc.RO) : GAKE_out_i = {
+module GAKEb_st (S: Server) (C: Client) (H : GAKEc.HROc.RO) : GAKE_nodhs_i = {
   var b0 : bool 
 
   var servers : (s_id, server_state) fmap
@@ -62,17 +62,6 @@ module GAKEb_st (S: Server) (C: Client) (H : GAKEc.HROc.RO) : GAKE_out_i = {
       servers.[b] <- Honest kp;
     }
     return omap get_pkey servers.[b];
-  }
-
-  proc set_cert(b: s_id, pk: pkey) : unit option = {
-    var r <- None;
-
-    if (b \notin servers) {
-      servers.[b] <- Dishonest pk;
-      pk_set <- pk_set `|` fset1 pk;
-      r <- Some ();
-    }
-    return r;
   }
 
   proc send_msg1(i: int, m1: s_id) : pkey option = {
@@ -346,18 +335,18 @@ module GAKEb_st (S: Server) (C: Client) (H : GAKEc.HROc.RO) : GAKE_out_i = {
 require import NTOR_nosid.
 import GAKE_mod.
 
-op rem_sid_c (s : pr_st_client GAKEc.instance_state) : pr_st_client_mod instance_state =
+op rem_sid_c (s : GAKEc.pr_st_client GAKEc.instance_state) : pr_st_client instance_state =
 match s with 
-| GAKEc.Pending st pt ir => GAKE_mod.Pending (st.`2, st.`3) pt.`2 ir
-| GAKEc.Accepted st t k ir => GAKE_mod.Accepted (st.`2, st.`3) ((t.`1).`2, t.`2) k ir
-| GAKEc.Aborted st t ir => GAKE_mod.Aborted (Some ((oget st).`2, (oget st).`3)) (Some (((oget t).`1).`2, (oget t).`2)) ir
+| GAKEc.Pending st pt ir => GAKE_mod.Pending (st.`2, st.`3) (st.`2, pt.`2) ir
+| GAKEc.Accepted st t k ir => GAKE_mod.Accepted (st.`2, st.`3) ((st.`2, (t.`1).`2), t.`2) k ir
+| GAKEc.Aborted st t ir => GAKE_mod.Aborted (Some ((oget st).`2, (oget st).`3)) (Some (((oget st).`2, ((oget t).`1).`2), (oget t).`2)) ir
 end.
 
-op rem_sid_s (s : pr_st_server GAKEc.instance_state) : pr_st_server_mod instance_state =
+op rem_sid_s (s : GAKEc.pr_st_server GAKEc.instance_state) : pr_st_server instance_state =
 match s with 
-| GAKEc.Pending st pt ir => GAKE_mod.Pending (st.`2, st.`3) pt.`2 ir
-| GAKEc.Accepted st t k ir => GAKE_mod.Accepted (st.`2, st.`3) ((t.`1).`2, t.`2)k ir
-| GAKEc.Aborted st t ir => GAKE_mod.Aborted (Some ((oget st).`2, (oget st).`3)) (Some (((oget t).`1).`2, (oget t).`2)) ir
+| GAKEc.Pending st pt ir => GAKE_mod.Pending (st.`2, st.`3) (g ^ st.`2, pt.`2) ir
+| GAKEc.Accepted st t k ir => GAKE_mod.Accepted (st.`2, st.`3) ((g ^ st.`2, (t.`1).`2), t.`2) k ir
+| GAKEc.Aborted st t ir => GAKE_mod.Aborted (Some ((oget st).`2, (oget st).`3)) (Some ((g ^ (oget st).`2, ((oget t).`1).`2), (oget t).`2)) ir
 end.
 
 
@@ -380,205 +369,251 @@ op get_sr_in s_st : bool =
 with s_st = Inner _ bool => bool
 with s_st = Outer _ => true.
 
+module (Hon_Red (A : GAKEc.A_GAKE) : GAKEc.A_GAKE) (O : GAKEc.GAKE) = {
+  module O_GAKE : GAKEc.GAKE = {
+    var dh_ro : (pkey * pkey * s_id * pkey * pkey, (tag * key)) fmap
+    var c_inst : (int, bool) fmap
+    var dhc_smap : (int, GAKEc.pr_st_client GAKEc.instance_state) fmap
+    var servers : (s_id, server_state_mod) fmap
 
-module Hon_Red (O : GAKEc.GAKE_out_i) : GAKEc.GAKE_out_i = {
-  var dh_ro : (pkey * pkey * s_id * pkey * pkey, (tag * key)) fmap
-  var c_inst : (int, bool) fmap
-  var dhc_smap : (int, pr_st_client GAKEc.instance_state) fmap
-  var servers : (s_id, server_state_mod) fmap
+    proc h = O.h
 
-  proc init_mem(b: bool) = {
-    O.init_mem(b);
-    dhc_smap <- empty;
-    c_inst <- empty;
-    dh_ro <- empty;
-    servers <- empty;
-  }
-
-  proc h = O.h
-
-  proc init_s(b : s_id): pkey option = {
-  var r <- None;
-
-    r <@ O.init_s(b);
-    if (b \notin servers) {
-      servers.[b] <- Inner (oget r) false;
-    }
-
-    return r;
-  }
-
-  proc set_cert(b: s_id, pk: pkey) = { 
+    proc init_s(b : s_id): pkey option = {
     var r <- None;
 
-    r <@ O.set_cert(b, pk);
-    if (b \notin servers) {
-      servers.[b] <- Outer pk;
+      r <@ O.init_s(b);
+      if (b \notin servers) {
+        servers.[b] <- Inner (oget r) false;
+      }
+
+      return r;
     }
 
-    return r;
-  }
-
-  proc send_msg1(i: int, m1: s_id) = {
-    var sk_ce, pk_ce, pk_b; 
-    var r <- None;
-
-    if (m1 \in servers) {
-      if (!get_sr_out (oget servers.[m1]) /\ i \notin dhc_smap) {
-        r <@ O.send_msg1(i, m1);
-        if (r <> None) {
-          c_inst.[i] <- false;
-        }
-      } else {
-        if (i \notin c_inst) {
-          sk_ce <$ dt;
-          pk_ce <- g ^ sk_ce;
-          pk_b <- get_pkey_mod (oget servers.[m1]);
-          r <- Some pk_ce;
-          dhc_smap.[i] <- GAKEc.Pending (m1, pk_b, sk_ce) (m1, pk_ce) (false, false, false);
-          c_inst.[i] <- true;
+    proc set_cert(b: s_id, pk: pkey) = { 
+      var r <- None;
+  
+      r <@ O.set_cert(b, pk);
+      if (b \notin servers) {
+        servers.[b] <- Outer pk;
+      }
+  
+      return r;
+    }
+  
+    proc send_msg1(i: int, m1: s_id) = {
+      var sk_ce, pk_ce, pk_b; 
+      var r <- None;
+  
+      if (m1 \in servers) {
+        if (!get_sr_out (oget servers.[m1]) /\ i \notin dhc_smap) {
+          r <@ O.send_msg1(i, m1);
+          if (r <> None) {
+            c_inst.[i] <- false;
+          }
+        } else {
+          if (i \notin c_inst) {
+            sk_ce <$ dt;
+            pk_ce <- g ^ sk_ce;
+            pk_b <- get_pkey_mod (oget servers.[m1]);
+            r <- Some pk_ce;
+            dhc_smap.[i] <- GAKEc.Pending (m1, pk_b, sk_ce) (m1, pk_ce) (false, false, false);
+            c_inst.[i] <- true;
+          }
         }
       }
+  
+      return r;
     }
-
-    return r;
-  }
-
-  proc send_msg2 = O.send_msg2
-
-  proc send_msg3(i: int, m3: pkey * tag) = {
-    var pk_b, sk_ce, b, t_A, k;
-    var r <- None;
-
-    if (i \notin dhc_smap) {
-      r <@ O.send_msg3(i, m3);
-    } else {
-      match dhc_smap.[i] with 
-      | None => { } (* Abort? *)
-      | Some st => {
-          match st with
-          | GAKEc.Pending st pt ir => {
-              (b, pk_b, sk_ce) <- st;
-              (t_A, k) <@ O.h(m3.`1 ^ sk_ce, pk_b ^ sk_ce, b, g ^ sk_ce, m3.`1);
-              if (t_A = m3.`2) {
-                dhc_smap.[i] <- GAKEc.Accepted st (pt, Some m3) k ir;
-                r <- Some ();
-              } else {
-                dhc_smap.[i] <- GAKEc.Aborted (Some st) (Some (pt, Some m3)) ir;
+  
+    proc send_msg2 = O.send_msg2
+  
+    proc send_msg3(i: int, m3: pkey * tag) = {
+      var pk_b, sk_ce, b, t_A, k;
+      var r <- None;
+  
+      if (i \notin dhc_smap) {
+        r <@ O.send_msg3(i, m3);
+      } else {
+        match dhc_smap.[i] with 
+        | None => { } (* Abort? *)
+        | Some st => {
+            match st with
+            | GAKEc.Pending st pt ir => {
+                (b, pk_b, sk_ce) <- st;
+                (t_A, k) <@ O.h(m3.`1 ^ sk_ce, pk_b ^ sk_ce, b, g ^ sk_ce, m3.`1);
+                if (t_A = m3.`2) {
+                  dhc_smap.[i] <- GAKEc.Accepted st (pt, Some m3) k ir;
+                  r <- Some ();
+                } else {
+                  dhc_smap.[i] <- GAKEc.Aborted (Some st) (Some (pt, Some m3)) ir;
+                }
               }
-            }
-          | GAKEc.Accepted _ _ _ _ => { }
-          | GAKEc.Aborted _ _ _ => { }
-          end;
-        }
-      end;
+            | GAKEc.Accepted _ _ _ _ => { }
+            | GAKEc.Aborted _ _ _ => { }
+            end;
+          }
+        end;
+      }
+      return r;
     }
-    return r;
-  }
-
-  proc c_rev_skey(i: int) = {
-    var r <- None;
-
-    if (i \notin dhc_smap) {
-      r <@ O.c_rev_skey(i);
-    } else {
-      match dhc_smap.[i] with
-      | None => { }
-      | Some st => {
-          match st with 
-          | GAKEc.Pending _ _ _ => { }
-          | GAKEc.Accepted st' t' k' ir' => {
-              if (!get_ir_test (oget dhc_smap.[i])) { (* removed check on the partner and that they are untested, since an unhonest servers cannot be tested *)
-                r <- Some k';
-                dhc_smap.[i] <- set_ir_sess (GAKEc.Accepted st' t' k' ir');
+  
+    proc c_rev_skey(i: int) = {
+      var r <- None;
+  
+      if (i \notin dhc_smap) {
+        r <@ O.c_rev_skey(i);
+      } else {
+        match dhc_smap.[i] with
+        | None => { }
+        | Some st => {
+            match st with 
+            | GAKEc.Pending _ _ _ => { }
+            | GAKEc.Accepted st' t' k' ir' => {
+                if (!get_ir_test (oget dhc_smap.[i])) { (* removed check on the partner and that they are untested, since an unhonest servers cannot be tested *)
+                  r <- Some k';
+                  dhc_smap.[i] <- set_ir_sess (GAKEc.Accepted st' t' k' ir');
+                }
               }
-            }
-          | GAKEc.Aborted _ _ _ => { }
-          end;
-        }
-      end;
+            | GAKEc.Aborted _ _ _ => { }
+            end;
+          }
+        end;
+      }
+      return r;
     }
-    return r;
-  }
-
-  proc s_rev_skey(b: s_id, j: int) = {
-    var r <- None;
-
-    if (b \in servers /\ !get_sr_out (oget servers.[b])) {
-      r <@ O.s_rev_skey(b, j);
+  
+    proc s_rev_skey(b: s_id, j: int) = {
+      var r <- None;
+  
+      if (b \in servers /\ !get_sr_out (oget servers.[b])) {
+        r <@ O.s_rev_skey(b, j);
+      }
+  
+      return r;
     }
-
-    return r;
-  }
-
-  proc rev_ltkey(b: s_id) = {
-    var r <- None;
-
-    if (b \in servers /\ !get_sr_out (oget servers.[b])) {
-      r <@ O.rev_ltkey(b);
+  
+    proc rev_ltkey(b: s_id) = {
+      var r <- None;
+  
+      if (b \in servers /\ !get_sr_out (oget servers.[b])) {
+        r <@ O.rev_ltkey(b);
+      }
+  
+      return r;
     }
-
-    return r;
-  }
-
-  proc c_rev_ephkey(i : int) = {
-    var r <- None;
-
-    if (i \notin dhc_smap) {
-      r <@ O.c_rev_ephkey(i);
-    } else {
-      match dhc_smap.[i] with
-      | None => { }
-      | Some st => {
-          match st with
-          | GAKEc.Pending st pk_e ir => {
-              r <- Some (get_eph_c st);
-              dhc_smap.[i] <- set_ir_eph (GAKEc.Pending st pk_e ir);
-            }
-          | GAKEc.Accepted st t k ir => {
-              if (!get_ir_test (oget dhc_smap.[i])) {
+  
+    proc c_rev_ephkey(i : int) = {
+      var r <- None;
+  
+      if (i \notin dhc_smap) {
+        r <@ O.c_rev_ephkey(i);
+      } else {
+        match dhc_smap.[i] with
+        | None => { }
+        | Some st => {
+            match st with
+            | GAKEc.Pending st pk_e ir => {
                 r <- Some (get_eph_c st);
-                dhc_smap.[i] <- set_ir_eph (GAKEc.Accepted st t k ir);
+                dhc_smap.[i] <- set_ir_eph (GAKEc.Pending st pk_e ir);
               }
-            }
-          | GAKEc.Aborted _ _ _ => {  }
-           end;
-        }
-      end;
+            | GAKEc.Accepted st t k ir => {
+                if (!get_ir_test (oget dhc_smap.[i])) {
+                  r <- Some (get_eph_c st);
+                  dhc_smap.[i] <- set_ir_eph (GAKEc.Accepted st t k ir);
+                }
+              }
+            | GAKEc.Aborted _ _ _ => {  }
+             end;
+          }
+        end;
+      }
+  
+      return r;
     }
-
-    return r;
+  
+    proc s_rev_ephkey(b: s_id, j: int) = {
+      var r <- None;
+  
+      if (b \in servers /\ !get_sr_out (oget servers.[b])) {
+        r <@ O.s_rev_ephkey(b, j);
+      }
+  
+      return r;
+    }
+  
+    proc c_test(i : int) = {
+      var r <- None;
+  
+  
+      if (i \notin dhc_smap) {
+        r <@ O.c_test(i);
+      }
+  
+      return r;
+    }
+  
+    proc s_test(b: s_id, j: int) = {
+      var r <- None;
+  
+      if (b \in servers /\ !get_sr_out (oget servers.[b])) {
+        r <@ O.s_test(b, j);
+      }
+  
+      return r;
+    }
   }
 
-  proc s_rev_ephkey(b: s_id, j: int) = {
-    var r <- None;
+  proc run() : bool = {
+    var b';
 
-    if (b \in servers /\ !get_sr_out (oget servers.[b])) {
-      r <@ O.s_rev_ephkey(b, j);
+    O_GAKE.dhc_smap <- empty;
+    O_GAKE.c_inst <- empty;
+    O_GAKE.dh_ro <- empty;
+    O_GAKE.servers <- empty;
+
+    b' <@ A(O_GAKE).run();
+
+    return b';
+  }
+}.
+
+module (Hon_s_Red (A : GAKEc.A_GAKE) : GAKEc.A_GAKE_nodhs) (O : GAKEc.GAKE_nodhs) = {
+  module O_GAKE : GAKEc.GAKE = {
+    var servers : (s_id, (bool * pkey option)) fmap
+
+    include O [-init_s]
+
+    proc init_s(b : s_id) = {
+      var r;
+
+      if (b \notin servers) {
+        r <@ O.init_s(b);
+        servers.[b] <- (false, r);
+      }
+
+      return (oget servers.[b]).`2;
     }
 
-    return r;
+    proc set_cert(b: s_id, pk: pkey) = { 
+      var r <- None;
+  
+      if (b \notin servers) {
+        servers.[b] <- (true, Some pk);
+        r <- Some ();
+      }
+  
+      return r;
+    }
   }
 
-  proc c_test(i : int) = {
-    var r <- None;
+  proc run() : bool = {
+    var b';
 
+    O_GAKE.servers <- empty;
 
-    if (i \notin dhc_smap) {
-      r <@ O.c_test(i);
-    }
+    b' <@ A(O_GAKE).run();
 
-    return r;
-  }
-
-  proc s_test(b: s_id, j: int) = {
-    var r <- None;
-
-    if (b \in servers /\ !get_sr_out (oget servers.[b])) {
-      r <@ O.s_test(b, j);
-    }
-
-    return r;
+    return b';
   }
 }.
 
@@ -586,8 +621,8 @@ module Hon_Red (O : GAKEc.GAKE_out_i) : GAKEc.GAKE_out_i = {
 (* ------------------------------------------------------------------------------------------ *)
 (* Reduction preventing collisions and prediction of public keys  *)
 
-module (Name_Red (A : GAKEc.A_GAKE) : GAKE_mod.A_GAKE) (O : GAKE_mod.GAKE_out) = {
-  module O_GAKE : GAKEc.GAKE_out = {
+module (Name_Red (A : GAKEc.A_GAKE_nodhs) : GAKE_mod.A_GAKE_nodhs) (O : GAKE_mod.GAKE_nodhs) = {
+  module O_GAKE : GAKEc.GAKE_nodhs = {
     var unreg_ro : (pkey * pkey * s_id * pkey * pkey, (tag * key)) fmap
 
     var sid_pk : (s_id, server_state_mod) fmap
@@ -645,18 +680,6 @@ module (Name_Red (A : GAKEc.A_GAKE) : GAKE_mod.A_GAKE) (O : GAKE_mod.GAKE_out) =
         }
         r <- Some (get_pkey_mod (oget sid_pk.[b]));
       }
-      return r;
-    }
-
-    proc set_cert(b: s_id, pk: pkey) = {
-      var r <- None;
-
-      if (!stop /\ b \notin sid_pk) {
-        sid_pk.[b] <- Outer pk;
-        pk_set <- pk_set `|` fset1 pk;
-        r <- Some ();
-      }
-
       return r;
     }
 
@@ -836,9 +859,9 @@ module (Name_Red (A : GAKEc.A_GAKE) : GAKE_mod.A_GAKE) (O : GAKE_mod.GAKE_out) =
 (* ------------------------------------------------------------------------------------------ *)
 section.
 
-declare module A <: GAKEc.A_GAKE {-GAKE_mod.HROc.RO, -GAKEc.HROc.RO, -Hon_Red, -Name_Red, -GAKEc.GAKEb, -GAKEc.GAKEb_hon, -GAKEb_st, -GAKE_mod.GAKEb }.
+declare module A <: GAKEc.A_GAKE {-GAKE_mod.HROc.RO, -GAKEc.HROc.RO, -Hon_Red, -Hon_s_Red, -Name_Red, -GAKEc.GAKEb, -GAKEc.GAKEb_hon, -GAKEc.GAKEb_nodhs, -GAKEb_st, -GAKE_mod.GAKEb_nodhs }.
 
-declare axiom A_ll (G <: GAKEc.GAKE_out{-A}):
+declare axiom A_ll (G <: GAKEc.GAKE{-A}):
   islossless G.h =>
   islossless G.init_s =>
   islossless G.set_cert =>
@@ -855,35 +878,35 @@ declare axiom A_ll (G <: GAKEc.GAKE_out{-A}):
   islossless A(G).run. 
  
  
-lemma gake_hon bit &m: Pr[GAKEc.E_GAKE(GAKEc.GAKEb(NTOR_S(GAKEc.HROc.RO), NTOR_C(GAKEc.HROc.RO), GAKEc.HROc.RO), A).run(bit) @ &m : res] = Pr[GAKEc.E_GAKE(Hon_Red(GAKEc.GAKEb_hon(NTOR_S(GAKEc.HROc.RO), NTOR_C(GAKEc.HROc.RO), GAKEc.HROc.RO)), A).run(bit) @ &m : res].
+lemma gake_hon bit &m: Pr[GAKEc.E_GAKE(GAKEc.GAKEb(NTOR_S(GAKEc.HROc.RO), NTOR_C(GAKEc.HROc.RO), GAKEc.HROc.RO), A).run(bit) @ &m : res] = Pr[GAKEc.E_GAKE(GAKEc.GAKEb_hon(NTOR_S(GAKEc.HROc.RO), NTOR_C(GAKEc.HROc.RO), GAKEc.HROc.RO), Hon_Red(A)).run(bit) @ &m : res].
 proof.
 byequiv => //.
 proc; inline. admit. (*
 wp; call (: ={b0, servers, s_smap, tested}(GAKEc.GAKEb, GAKEc.GAKEb_hon) /\ ={m}(GAKEc.HROc.RO, GAKEc.HROc.RO)
   
-              /\ (GAKEc.GAKEb.c_smap{1} = (GAKEc.GAKEb_hon.c_smap{2} + Hon_Red.dhc_smap{2}))
-              /\ (forall i, i \in Hon_Red.dhc_smap{2} => i \notin GAKEc.GAKEb_hon.c_smap{2})
-              /\ (forall i, i \in GAKEc.GAKEb_hon.c_smap{2} => i \notin Hon_Red.dhc_smap{2})
-              /\ (forall b, b \in Hon_Red.servers{2} <=> b \in GAKEc.GAKEb_hon.servers{2})
+              /\ (GAKEc.GAKEb.c_smap{1} = (GAKEc.GAKEb_hon.c_smap{2} + Hon_Red.O_GAKE.dhc_smap{2}))
+              /\ (forall i, i \in Hon_Red.O_GAKE.dhc_smap{2} => i \notin GAKEc.GAKEb_hon.c_smap{2})
+              /\ (forall i, i \in GAKEc.GAKEb_hon.c_smap{2} => i \notin Hon_Red.O_GAKE.dhc_smap{2})
+              /\ (forall b, b \in Hon_Red.O_GAKE.servers{2} <=> b \in GAKEc.GAKEb_hon.servers{2})
               /\ (forall b, b \in GAKEc.GAKEb_hon.servers{2} 
-                   => get_pkey (oget GAKEc.GAKEb_hon.servers{2}.[b]) = get_pkey_mod (oget Hon_Red.servers{2}.[b])
-                                      /\ (get_sr_out (oget Hon_Red.servers{2}.[b]) = get_sr_dh (oget GAKEc.GAKEb_hon.servers{2}.[b])))
-              /\ (forall i, i \in GAKEc.GAKEb.c_smap{1} <=> i \in Hon_Red.c_inst{2})
-              /\ (forall i, i \in Hon_Red.dhc_smap{2} => get_ir_test (oget Hon_Red.dhc_smap{2}.[i]) = false
-                                       /\ get_name (oget Hon_Red.dhc_smap{2}.[i]) \in GAKEb_hon.servers{2}
-                                       /\ get_sr_dh (oget GAKEb_hon.servers{2}.[get_name (oget Hon_Red.dhc_smap{2}.[i])]))
+                   => get_pkey (oget GAKEc.GAKEb_hon.servers{2}.[b]) = get_pkey_mod (oget Hon_Red.O_GAKE.servers{2}.[b])
+                                      /\ (get_sr_out (oget Hon_Red.O_GAKE.servers{2}.[b]) = get_sr_dh (oget GAKEc.GAKEb_hon.servers{2}.[b])))
+              /\ (forall i, i \in GAKEc.GAKEb.c_smap{1} <=> i \in Hon_Red.O_GAKE.c_inst{2})
+              /\ (forall i, i \in Hon_Red.O_GAKE.dhc_smap{2} => get_ir_test (oget Hon_Red.O_GAKE.dhc_smap{2}.[i]) = false
+                                       /\ get_name (oget Hon_Red.O_GAKE.dhc_smap{2}.[i]) \in GAKEb_hon.servers{2}
+                                       /\ get_sr_dh (oget GAKEb_hon.servers{2}.[get_name (oget Hon_Red.O_GAKE.dhc_smap{2}.[i])]))
               /\ (forall b j , b \notin GAKEc.GAKEb_hon.servers{2} => (b, j) \notin GAKEc.GAKEb_hon.s_smap{2})
               /\ (forall b j, (b, j) \in GAKEc.GAKEb_hon.s_smap{2} => get_name (oget GAKEc.GAKEb_hon.s_smap{2}.[(b, j)]) = b
                                        /\ (exists pk m3, get_trace (oget GAKEc.GAKEb_hon.s_smap{2}.[(b, j)]) = Some ((b, pk), Some m3)))
               /\ (forall b j, b \in GAKEc.GAKEb_hon.servers{2} => get_sr_dh (oget GAKEc.GAKEb_hon.servers{2}.[b])
                    => (b, j) \notin GAKEc.GAKEb_hon.s_smap{2} /\ get_sr_ltk (oget GAKEc.GAKEb_hon.servers{2}.[b]))
-              /\ (forall i j, i \in Hon_Red.dhc_smap{2}  
-                   => (get_name (oget Hon_Red.dhc_smap{2}.[i]), j) \notin GAKEc.GAKEb_hon.s_smap{2})
-              /\ (forall i st pt ir m3, i \in Hon_Red.dhc_smap{2} => Hon_Red.dhc_smap{2}.[i] = Some (Pending st pt ir)
+              /\ (forall i j, i \in Hon_Red.O_GAKE.dhc_smap{2}  
+                   => (get_name (oget Hon_Red.O_GAKE.dhc_smap{2}.[i]), j) \notin GAKEc.GAKEb_hon.s_smap{2})
+              /\ (forall i st pt ir m3, i \in Hon_Red.O_GAKE.dhc_smap{2} => Hon_Red.O_GAKE.dhc_smap{2}.[i] = Some (Pending st pt ir)
                    => (1 <= card (get_partners_c (pt, Some m3) GAKEc.GAKEb_hon.s_smap{2})) = false)
-              /\ (forall i st pt ir, i \in Hon_Red.dhc_smap{2} => Hon_Red.dhc_smap{2}.[i{2}] = Some (Pending st pt ir)
+              /\ (forall i st pt ir, i \in Hon_Red.O_GAKE.dhc_smap{2} => Hon_Red.O_GAKE.dhc_smap{2}.[i{2}] = Some (Pending st pt ir)
                    => (1 <= card (get_origins_c (pt, None) GAKEc.GAKEb_hon.s_smap{2}) = false))
-              /\ (forall i st t k ir, i \in Hon_Red.dhc_smap{2} => Hon_Red.dhc_smap{2}.[i] = Some (Accepted st t k ir)
+              /\ (forall i st t k ir, i \in Hon_Red.O_GAKE.dhc_smap{2} => Hon_Red.O_GAKE.dhc_smap{2}.[i] = Some (Accepted st t k ir)
                    => (1 <= card (get_partners_c t GAKEc.GAKEb_hon.s_smap{2})) = false)).
 
 + sim />.
@@ -917,12 +940,12 @@ wp; call (: ={b0, servers, s_smap, tested}(GAKEc.GAKEb, GAKEc.GAKEb_hon) /\ ={m}
         rewrite get_setE //=.
         move => [#] steq pteq ireq.
         rewrite /get_partners_c.
-        case ((i{2} \notin Hon_Red.dhc_smap{2})) => indhc; 2: by smt(get_setE mem_set in_fsetU in_fset1 joinE).
-        have->: (fdom (filter (fun (_ : s_id * int) (val : pr_st_server GAKEc.instance_state) => get_trace val = Some (pt, Some m3)) GAKEb_hon.s_smap{2})) = fset0.
+        case ((i{2} \notin Hon_Red.O_GAKE.dhc_smap{2})) => indhc; 2: by smt(get_setE mem_set in_fsetU in_fset1 joinE).
+        have->: (fdom (filter (fun (_ : s_id * int) (val : GAKEc.pr_st_server GAKEc.instance_state) => get_trace val = Some (pt, Some m3)) GAKEb_hon.s_smap{2})) = fset0.
         + rewrite fsetP.
           move => x.
           rewrite mem_fdom mem_filter.
-          have->: !(x \in GAKEb_hon.s_smap{2} /\ (fun (_ : s_id * int) (val : pr_st_server GAKEc.instance_state) =>
+          have->: !(x \in GAKEb_hon.s_smap{2} /\ (fun (_ : s_id * int) (val : GAKEc.pr_st_server GAKEc.instance_state) =>
               get_trace val = Some (pt, Some m3)) x (oget GAKEb_hon.s_smap{2}.[x])).
           + rewrite negb_and.
             case (x \in GAKEb_hon.s_smap{2}); 2: by smt().
@@ -940,13 +963,13 @@ wp; call (: ={b0, servers, s_smap, tested}(GAKEc.GAKEb, GAKEc.GAKEb_hon) /\ ={m}
         rewrite get_setE //=.
         move => [#] steq pteq ireq.
         rewrite /get_origins_c.
-        case ((i{2} \notin Hon_Red.dhc_smap{2})) => indhc; 2: by smt(get_setE mem_set in_fsetU in_fset1 joinE).
-        have->: (fdom (filter (fun (_ : s_id * int) (val : pr_st_server GAKEc.instance_state) 
+        case ((i{2} \notin Hon_Red.O_GAKE.dhc_smap{2})) => indhc; 2: by smt(get_setE mem_set in_fsetU in_fset1 joinE).
+        have->: (fdom (filter (fun (_ : s_id * int) (val : GAKEc.pr_st_server GAKEc.instance_state) 
           => exists (m2o : (pkey * tag) option), get_trace val = Some (pt, m2o)) GAKEb_hon.s_smap{2})) = fset0.
         + rewrite fsetP.
           move => x.
           rewrite mem_fdom mem_filter. 
-          have->: !(x \in GAKEb_hon.s_smap{2} /\ (fun (_ : s_id * int) (val : pr_st_server GAKEc.instance_state) =>
+          have->: !(x \in GAKEb_hon.s_smap{2} /\ (fun (_ : s_id * int) (val : GAKEc.pr_st_server GAKEc.instance_state) =>
               exists (m2o : (pkey * tag) option), get_trace val = Some (pt, m2o)) x (oget GAKEb_hon.s_smap{2}.[x])).
           + rewrite negb_and.
             case (x \in GAKEb_hon.s_smap{2}); 2: by smt().
@@ -1110,14 +1133,14 @@ wp; call (: ={b0, servers, s_smap, tested}(GAKEc.GAKEb, GAKEc.GAKEb_hon) /\ ={m}
       + auto => /> &1 &2 *. 
         rewrite /untested_partner_s.
         rewrite /get_partners_s /get_untested_partners_s.
-        have->: (fdom (filter (fun (_ : int) (val : pr_st_client GAKEc.instance_state) => get_trace val = Some t) (GAKEb_hon.c_smap{1} + Hon_Red.dhc_smap{1}))) 
-            = (fdom (filter (fun (_ : int) (val : pr_st_client GAKEc.instance_state) => get_trace val = Some t) GAKEb_hon.c_smap{1})).
+        have->: (fdom (filter (fun (_ : int) (val : GAKEc.pr_st_client GAKEc.instance_state) => get_trace val = Some t) (GAKEb_hon.c_smap{1} + Hon_Red.O_GAKE.dhc_smap{1}))) 
+            = (fdom (filter (fun (_ : int) (val : GAKEc.pr_st_client GAKEc.instance_state) => get_trace val = Some t) GAKEb_hon.c_smap{1})).
         + rewrite fsetP.
           move => x.
           do rewrite mem_fdom mem_filter.
           by smt(joinE).
-        have->: (fdom (filter (fun (_ : int) (val : pr_st_client GAKEc.instance_state) => get_trace val = Some t /\ get_ir_test val = false)
-             (GAKEb_hon.c_smap{1} + Hon_Red.dhc_smap{1}))) = (fdom (filter (fun (_ : int) (val : pr_st_client GAKEc.instance_state) =>
+        have->: (fdom (filter (fun (_ : int) (val : GAKEc.pr_st_client GAKEc.instance_state) => get_trace val = Some t /\ get_ir_test val = false)
+             (GAKEb_hon.c_smap{1} + Hon_Red.O_GAKE.dhc_smap{1}))) = (fdom (filter (fun (_ : int) (val : GAKEc.pr_st_client GAKEc.instance_state) =>
                 get_trace val = Some t /\ get_ir_test val = false) GAKEb_hon.c_smap{1})). 
         + rewrite fsetP.
           move => x.
@@ -1163,20 +1186,20 @@ wp; call (: ={b0, servers, s_smap, tested}(GAKEc.GAKEb, GAKEc.GAKEb_hon) /\ ={m}
       if => //.
       + auto => /> &2 *.
         have : (forall b j t, (b, j) \in GAKEc.GAKEb_hon.s_smap{2} /\ t = (oget (get_trace (oget GAKEc.GAKEb_hon.s_smap{2}.[b, j])))
-            => get_untested_partners_s t (GAKEb_hon.c_smap{2} + Hon_Red.dhc_smap{2}) = get_untested_partners_s t GAKEc.GAKEb_hon.c_smap{2}
-            /\ get_partners_s t (GAKEb_hon.c_smap{2} + Hon_Red.dhc_smap{2}) = get_partners_s t GAKEc.GAKEb_hon.c_smap{2}).
+            => get_untested_partners_s t (GAKEb_hon.c_smap{2} + Hon_Red.O_GAKE.dhc_smap{2}) = get_untested_partners_s t GAKEc.GAKEb_hon.c_smap{2}
+            /\ get_partners_s t (GAKEb_hon.c_smap{2} + Hon_Red.O_GAKE.dhc_smap{2}) = get_partners_s t GAKEc.GAKEb_hon.c_smap{2}).
         + rewrite /untested_partner_s.
           rewrite /get_partners_s /get_untested_partners_s.
           move => b1 j t [] bjin teq.
-          have->: (fdom (filter (fun (_ : int) (val : pr_st_client GAKEc.instance_state) => get_trace val = Some t /\ get_ir_test val = false) (GAKEb_hon.c_smap{2} 
-              + Hon_Red.dhc_smap{2}))) = (fdom (filter (fun (_ : int) (val : pr_st_client GAKEc.instance_state) 
+          have->: (fdom (filter (fun (_ : int) (val : GAKEc.pr_st_client GAKEc.instance_state) => get_trace val = Some t /\ get_ir_test val = false) (GAKEb_hon.c_smap{2} 
+              + Hon_Red.O_GAKE.dhc_smap{2}))) = (fdom (filter (fun (_ : int) (val : GAKEc.pr_st_client GAKEc.instance_state) 
               => get_trace val = Some t /\ get_ir_test val = false) GAKEb_hon.c_smap{2})).
           + rewrite fsetP.
             move => x.
             do rewrite mem_fdom mem_filter.
             smt(joinE).
-          have->: (fdom (filter (fun (_ : int) (val : pr_st_client GAKEc.instance_state) => get_trace val = Some t) (GAKEb_hon.c_smap{2} + Hon_Red.dhc_smap{2}))) = 
-              (fdom (filter (fun (_ : int) (val : pr_st_client GAKEc.instance_state) => get_trace val = Some t) GAKEb_hon.c_smap{2})). 
+          have->: (fdom (filter (fun (_ : int) (val : GAKEc.pr_st_client GAKEc.instance_state) => get_trace val = Some t) (GAKEb_hon.c_smap{2} + Hon_Red.O_GAKE.dhc_smap{2}))) = 
+              (fdom (filter (fun (_ : int) (val : GAKEc.pr_st_client GAKEc.instance_state) => get_trace val = Some t) GAKEb_hon.c_smap{2})). 
           + rewrite fsetP.
             move => x.
             do rewrite mem_fdom mem_filter.
@@ -1232,14 +1255,14 @@ wp; call (: ={b0, servers, s_smap, tested}(GAKEc.GAKEb, GAKEc.GAKEb_hon) /\ ={m}
       + auto => /> &1 &2 *. 
         rewrite /untested_partner_s.
         rewrite /get_partners_s /get_untested_partners_s.
-        have->: (fdom (filter (fun (_ : int) (val : pr_st_client GAKEc.instance_state) => get_trace val = Some t) (GAKEb_hon.c_smap{1} + Hon_Red.dhc_smap{1}))) 
-          = (fdom (filter (fun (_ : int) (val : pr_st_client GAKEc.instance_state) => get_trace val = Some t) GAKEb_hon.c_smap{1})).
+        have->: (fdom (filter (fun (_ : int) (val : GAKEc.pr_st_client GAKEc.instance_state) => get_trace val = Some t) (GAKEb_hon.c_smap{1} + Hon_Red.O_GAKE.dhc_smap{1}))) 
+          = (fdom (filter (fun (_ : int) (val : GAKEc.pr_st_client GAKEc.instance_state) => get_trace val = Some t) GAKEb_hon.c_smap{1})).
         + rewrite fsetP.
           move => x.
           do rewrite mem_fdom mem_filter.
           by smt(joinE).
-        have->: (fdom (filter (fun (_ : int) (val : pr_st_client GAKEc.instance_state) => get_trace val = Some t /\ get_ir_test val = false)
-             (GAKEb_hon.c_smap{1} + Hon_Red.dhc_smap{1}))) = (fdom (filter (fun (_ : int) (val : pr_st_client GAKEc.instance_state) =>
+        have->: (fdom (filter (fun (_ : int) (val : GAKEc.pr_st_client GAKEc.instance_state) => get_trace val = Some t /\ get_ir_test val = false)
+             (GAKEb_hon.c_smap{1} + Hon_Red.O_GAKE.dhc_smap{1}))) = (fdom (filter (fun (_ : int) (val : GAKEc.pr_st_client GAKEc.instance_state) =>
                 get_trace val = Some t /\ get_ir_test val = false) GAKEb_hon.c_smap{1})). 
         + rewrite fsetP.
           move => x.
@@ -1313,16 +1336,16 @@ wp; call (: ={b0, servers, s_smap, tested}(GAKEc.GAKEb, GAKEc.GAKEb_hon) /\ ={m}
         + auto => /> &1 &2 *.
           rewrite /fresh_partner_s.
           rewrite /get_origins_s /get_fresh_partners_s.
-          have->: (fdom (filter (fun (_ : int) (val : pr_st_client GAKEc.instance_state) =>
-               exists (m2o : (pkey * tag) option), get_trace val = Some (t.`1, m2o)) (GAKEb_hon.c_smap{1} + Hon_Red.dhc_smap{1}))) = (fdom
-               (filter (fun (_ : int) (val : pr_st_client GAKEc.instance_state) => exists (m2o : (pkey * tag) option), get_trace val = Some (t.`1, m2o)) GAKEb_hon.c_smap{1})).
+          have->: (fdom (filter (fun (_ : int) (val : GAKEc.pr_st_client GAKEc.instance_state) =>
+               exists (m2o : (pkey * tag) option), get_trace val = Some (t.`1, m2o)) (GAKEb_hon.c_smap{1} + Hon_Red.O_GAKE.dhc_smap{1}))) = (fdom
+               (filter (fun (_ : int) (val : GAKEc.pr_st_client GAKEc.instance_state) => exists (m2o : (pkey * tag) option), get_trace val = Some (t.`1, m2o)) GAKEb_hon.c_smap{1})).
           + rewrite fsetP.
             move => x.
             do rewrite mem_fdom mem_filter.
             by smt(joinE).
-          have->: (fdom (filter (fun (_ : int) (val : pr_st_client GAKEc.instance_state) =>
+          have->: (fdom (filter (fun (_ : int) (val : GAKEc.pr_st_client GAKEc.instance_state) =>
                   (exists (m2o : (pkey * tag) option), get_trace val = Some (t.`1, m2o)) /\ get_ir_test val = false /\ get_ir_sess val = false /\ get_ir_eph val = false)
-               (GAKEb_hon.c_smap{1} + Hon_Red.dhc_smap{1}))) = (fdom (filter (fun (_ : int) (val : pr_st_client GAKEc.instance_state) =>
+               (GAKEb_hon.c_smap{1} + Hon_Red.O_GAKE.dhc_smap{1}))) = (fdom (filter (fun (_ : int) (val : GAKEc.pr_st_client GAKEc.instance_state) =>
                   (exists (m2o : (pkey * tag) option), get_trace val = Some (t.`1, m2o)) /\ get_ir_test val = false /\ get_ir_sess val = false /\ get_ir_eph val = false)
                GAKEb_hon.c_smap{1})). 
           + rewrite fsetP.
@@ -1399,32 +1422,70 @@ wp; call (: ={b0, servers, s_smap, tested}(GAKEc.GAKEb, GAKEc.GAKEb_hon) /\ ={m}
   match None {1} ^match. auto => /#.
   auto => />.
 
-auto => />; smt(fmap_eqP joinE mem_empty emptyE).*)
+auto => />; smt(fmap_eqP joinE mem_empty emptyE). *)
 qed.
 
-
-lemma gake_st bit &m: Pr[GAKEc.E_GAKE(GAKEb_hon(NTOR_S(GAKEc.HROc.RO), NTOR_C(GAKEc.HROc.RO), GAKEc.HROc.RO), A).run(bit) @ &m : res] 
-                = Pr[GAKEc.E_GAKE(GAKEb_st(NTOR_S(GAKEc.HROc.RO), NTOR_C(GAKEc.HROc.RO), GAKEc.HROc.RO), A).run(bit) @ &m : res].
+lemma rem_dhs bit &m: Pr[GAKEc.E_GAKE(GAKEc.GAKEb_hon(NTOR_S(GAKEc.HROc.RO), NTOR_C(GAKEc.HROc.RO), GAKEc.HROc.RO), A).run(bit) @ &m : res] = 
+  Pr[GAKEc.E_GAKE_nodhs(GAKEc.GAKEb_nodhs(NTOR_S(GAKEc.HROc.RO), NTOR_C(GAKEc.HROc.RO), GAKEc.HROc.RO), Hon_s_Red(A)).run(bit) @ &m : res].
 proof.
 byequiv => //.
 proc; inline.
-call (: ={b0, servers, c_smap, s_smap, tested}(GAKEb_hon, GAKEb_st) /\ ={m}(GAKEc.HROc.RO, GAKEc.HROc.RO)); try sim />.
+wp; call (: ={b0, c_smap, s_smap, tested}(GAKEb_hon, GAKEc.GAKEb_nodhs) /\ ={m}(GAKEc.HROc.RO, GAKEc.HROc.RO)
+               /\ (forall b, b \in GAKEb_hon.servers{1} <=> b \in Hon_s_Red.O_GAKE.servers{2})
+               /\ (forall b, b \notin Hon_s_Red.O_GAKE.servers{2} => b \notin GAKEc.GAKEb_nodhs.servers{2})
+               /\ (forall b, b \in Hon_s_Red.O_GAKE.servers{2} => (oget Hon_s_Red.O_GAKE.servers{2}.[b]).`1 = false
+                   => GAKEb_hon.servers{1}.[b] = GAKEc.GAKEb_nodhs.servers{2}.[b])
+               /\ (forall b, b \in Hon_s_Red.O_GAKE.servers{2} => omap get_pkey GAKEb_hon.servers{1}.[b] = (oget Hon_s_Red.O_GAKE.servers{2}.[b]).`2)
+      ); 1,6,7,8,10: sim />.
+
++ proc; inline.
+  if => //. auto => /#.
+  + rcondt {2} ^if. auto => /#.
+    auto => />; smt(get_setE mem_set).
+  auto => /> &1 &2 *. smt(get_setE mem_set).
+
++ proc; inline.
+  sp 1 1; if => //. auto => /#.
+  auto => /> &1 &2 *. smt(get_setE mem_set).
+
+admit. 
+
+admit.
+
+admit.
+
+admit.
+
+admit.
+
+admit. 
+
+auto => />. smt(mem_empty emptyE).
+qed.
+
+
+lemma gake_st bit &m: Pr[GAKEc.E_GAKE_nodhs(GAKEc.GAKEb_nodhs(NTOR_S(GAKEc.HROc.RO), NTOR_C(GAKEc.HROc.RO), GAKEc.HROc.RO), Hon_s_Red(A)).run(bit) @ &m : res] 
+                = Pr[GAKEc.E_GAKE_nodhs(GAKEb_st(NTOR_S(GAKEc.HROc.RO), NTOR_C(GAKEc.HROc.RO), GAKEc.HROc.RO), Hon_s_Red(A)).run(bit) @ &m : res].
+proof.
+byequiv => //.
+proc; inline.
+wp; call (: ={b0, servers, c_smap, s_smap, tested}(GAKEc.GAKEb_nodhs, GAKEb_st) /\ ={servers}(Hon_s_Red.O_GAKE, Hon_s_Red.O_GAKE) /\ ={m}(GAKEc.HROc.RO, GAKEc.HROc.RO)); try sim />.
 
 + proc; inline.
   auto => />.
 qed.
 
 
-lemma gake_st_mod bit &m: `| Pr[GAKEc.E_GAKE(GAKEb_st(NTOR_S(GAKEc.HROc.RO), NTOR_C(GAKEc.HROc.RO), GAKEc.HROc.RO), A).run(bit) @ &m : res]
-                 - Pr[GAKE_mod.E_GAKE(GAKE_mod.GAKEb(NTOR_S_mod(GAKE_mod.HROc.RO), NTOR_C_mod(GAKE_mod.HROc.RO), GAKE_mod.HROc.RO), Name_Red(A)).run(bit) @ &m : res] | 
-                     <= Pr[GAKEc.E_GAKE(GAKEb_st(NTOR_S(GAKEc.HROc.RO), NTOR_C(GAKEc.HROc.RO), GAKEc.HROc.RO), A).run(bit) @ &m : GAKEb_st.stop].
+lemma gake_st_mod bit &m: `| Pr[GAKEc.E_GAKE_nodhs(GAKEb_st(NTOR_S(GAKEc.HROc.RO), NTOR_C(GAKEc.HROc.RO), GAKEc.HROc.RO), Hon_s_Red(A)).run(bit) @ &m : res]
+     - Pr[GAKE_mod.E_GAKE_nodhs(GAKE_mod.GAKEb_nodhs(NTOR_S_mod(GAKE_mod.HROc.RO), NTOR_C_mod(GAKE_mod.HROc.RO), GAKE_mod.HROc.RO), Name_Red(Hon_s_Red(A))).run(bit) @ &m : res] | 
+                 <= Pr[GAKEc.E_GAKE_nodhs(GAKEb_st(NTOR_S(GAKEc.HROc.RO), NTOR_C(GAKEc.HROc.RO), GAKEc.HROc.RO), Hon_s_Red(A)).run(bit) @ &m : GAKEb_st.stop].
 proof.
 rewrite StdOrder.RealOrder.distrC.
 byequiv (: _ ==> _) : Name_Red.O_GAKE.stop => //; first last.
 + smt().
 symmetry; proc; inline*.
 wp; call (: Name_Red.O_GAKE.stop
-          , ={b0, tested}(GAKEb_st, GAKE_mod.GAKEb) /\ ={pk_set, stop}(GAKEb_st, Name_Red.O_GAKE)
+          , ={b0, tested}(GAKEb_st, GAKE_mod.GAKEb_nodhs) /\ ={pk_set, stop}(GAKEb_st, Name_Red.O_GAKE) /\ ={servers}(Hon_s_Red.O_GAKE, Hon_s_Red.O_GAKE)
 
                /\ (forall x, x \in GAKEc.HROc.RO.m{1} => x.`3 \in Name_Red.O_GAKE.sid_pk{2} => !get_sr_out (oget Name_Red.O_GAKE.sid_pk{2}.[x.`3]) 
                     => x \notin Name_Red.O_GAKE.unreg_ro{2}
@@ -1444,16 +1505,16 @@ wp; call (: Name_Red.O_GAKE.stop
                /\ (forall x, x \in GAKEc.HROc.RO.m{1} => x.`4 \in Name_Red.O_GAKE.pk_set{2} /\ x.`5 \in Name_Red.O_GAKE.pk_set{2})
                /\ (forall x, x \in GAKE_mod.HROc.RO.m{2} => x.`4 \in Name_Red.O_GAKE.pk_set{2} /\ x.`5 \in Name_Red.O_GAKE.pk_set{2})
 
-               /\ (forall i, i \in GAKEb_st.c_smap{1} <=> i \in GAKE_mod.GAKEb.c_smap{2})
+               /\ (forall i, i \in GAKEb_st.c_smap{1} <=> i \in GAKE_mod.GAKEb_nodhs.c_smap{2})
 
-               /\ (forall i, i \in GAKE_mod.GAKEb.c_smap{2} => rem_sid_c (oget GAKEb_st.c_smap{1}.[i]) = oget GAKE_mod.GAKEb.c_smap{2}.[i])
+               /\ (forall i, i \in GAKE_mod.GAKEb_nodhs.c_smap{2} => rem_sid_c (oget GAKEb_st.c_smap{1}.[i]) = oget GAKE_mod.GAKEb_nodhs.c_smap{2}.[i])
 
                /\ (forall b j, (b, j) \in GAKEb_st.s_smap{1} => b \in Name_Red.O_GAKE.sid_pk{2} /\ !(get_sr_out (oget Name_Red.O_GAKE.sid_pk{2}.[b])
-                                     /\ (get_pkey_mod (oget Name_Red.O_GAKE.sid_pk{2}.[b]), j) \in GAKE_mod.GAKEb.s_smap{2}
-                                     /\ rem_sid_s (oget GAKEb_st.s_smap{1}.[(b, j)]) = oget GAKE_mod.GAKEb.s_smap{2}.[(get_pkey_mod (oget Name_Red.O_GAKE.sid_pk{2}.[b]), j)]))
+                                     /\ (get_pkey_mod (oget Name_Red.O_GAKE.sid_pk{2}.[b]), j) \in GAKE_mod.GAKEb_nodhs.s_smap{2}
+                                     /\ rem_sid_s (oget GAKEb_st.s_smap{1}.[(b, j)]) = oget GAKE_mod.GAKEb_nodhs.s_smap{2}.[(get_pkey_mod (oget Name_Red.O_GAKE.sid_pk{2}.[b]), j)]))
 
                /\ (forall b j, b \in Name_Red.O_GAKE.sid_pk{2} => !get_sr_out (oget Name_Red.O_GAKE.sid_pk{2}.[b])
-                    => (get_pkey_mod (oget Name_Red.O_GAKE.sid_pk{2}.[b]), j) \in GAKE_mod.GAKEb.s_smap{2} 
+                    => (get_pkey_mod (oget Name_Red.O_GAKE.sid_pk{2}.[b]), j) \in GAKE_mod.GAKEb_nodhs.s_smap{2} 
                     <=> (b, j) \in GAKEb_st.s_smap{1})
 
                /\ (forall b, b \in GAKEb_st.servers{1} <=> b \in Name_Red.O_GAKE.sid_pk{2})
@@ -1464,11 +1525,11 @@ wp; call (: Name_Red.O_GAKE.stop
 
                /\ (forall b kp, b \in GAKEb_st.servers{1} => oget GAKEb_st.servers{1}.[b] = Honest kp
                     => b \in Name_Red.O_GAKE.sid_pk{2} /\ oget Name_Red.O_GAKE.sid_pk{2}.[b] = Inner kp.`1 false 
-                                      /\ kp.`1 \in GAKE_mod.GAKEb.servers{2} /\ oget GAKE_mod.GAKEb.servers{2}.[kp.`1] = Honest kp.`2)
+                                      /\ kp.`1 \in GAKE_mod.GAKEb_nodhs.servers{2} /\ oget GAKE_mod.GAKEb_nodhs.servers{2}.[kp.`1] = Honest kp.`2)
 
                /\ (forall b kp, b \in GAKEb_st.servers{1} => oget GAKEb_st.servers{1}.[b] = Corrupt kp
                     => b \in Name_Red.O_GAKE.sid_pk{2} /\ oget Name_Red.O_GAKE.sid_pk{2}.[b] = Inner kp.`1 true 
-                                      /\ kp.`1 \in GAKE_mod.GAKEb.servers{2} /\ oget GAKEb.servers{2}.[kp.`1] = Corrupt kp.`2)
+                                      /\ kp.`1 \in GAKE_mod.GAKEb_nodhs.servers{2} /\ oget GAKEb_nodhs.servers{2}.[kp.`1] = Corrupt kp.`2)
 
                /\ (forall b pk, b \in GAKEb_st.servers{1} => oget GAKEb_st.servers{1}.[b] = Dishonest pk
                     => b \in Name_Red.O_GAKE.sid_pk{2} /\ oget Name_Red.O_GAKE.sid_pk{2}.[b] = Outer pk)
@@ -1476,9 +1537,9 @@ wp; call (: Name_Red.O_GAKE.stop
                /\ (forall b, b \in GAKEb_st.servers{1} => obind get_skey GAKEb_st.servers{1}.[b] = None 
                    <=> oget Name_Red.O_GAKE.sid_pk{2}.[b] = Outer (get_pkey (oget GAKEb_st.servers{1}.[b])))
 
-               /\ (forall b, b \in GAKEb_st.servers{1} => !get_sr_dh (oget GAKEb_st.servers{1}.[b]) => get_pkey (oget GAKEb_st.servers{1}.[b]) \in GAKEb.servers{2})
+               /\ (forall b, b \in GAKEb_st.servers{1} => !get_sr_dh (oget GAKEb_st.servers{1}.[b]) => get_pkey (oget GAKEb_st.servers{1}.[b]) \in GAKEb_nodhs.servers{2})
 
-               /\ (forall pk b sk1 sk2, pk \in GAKEb.servers{2} => obind GAKE_mod.get_skey GAKEb.servers{2}.[pk] = Some sk1 
+               /\ (forall pk b sk1 sk2, pk \in GAKEb_nodhs.servers{2} => obind GAKE_mod.get_skey GAKEb_nodhs.servers{2}.[pk] = Some sk1 
                     => b \in GAKEb_st.servers{1} => obind GAKEc.get_skey GAKEb_st.servers{1}.[b] = Some sk2 
                     => b \in Name_Red.O_GAKE.sid_pk{2} => get_pkey_mod (oget Name_Red.O_GAKE.sid_pk{2}.[b]) = pk => sk1 = sk2)
 
@@ -1487,16 +1548,16 @@ wp; call (: Name_Red.O_GAKE.stop
                /\ (forall b, b \in Name_Red.O_GAKE.sid_pk{2} => !get_sr_in (oget Name_Red.O_GAKE.sid_pk{2}.[b]) => !get_sr_out (oget Name_Red.O_GAKE.sid_pk{2}.[b]))
 
                /\ (forall b pk bool, b \in Name_Red.O_GAKE.sid_pk{2} => oget Name_Red.O_GAKE.sid_pk{2}.[b] = Inner pk bool
-                    =>  obind GAKE_mod.get_skey GAKEb.servers{2}.[pk] <> None)
+                    =>  obind GAKE_mod.get_skey GAKEb_nodhs.servers{2}.[pk] <> None)
 
-               /\ (forall sk, g ^ sk \in GAKEb.servers{2} => obind GAKE_mod.get_skey GAKEb.servers{2}.[g ^ sk] = Some sk)
+               /\ (forall sk, g ^ sk \in GAKEb_nodhs.servers{2} => obind GAKE_mod.get_skey GAKEb_nodhs.servers{2}.[g ^ sk] = Some sk)
 
                /\ (forall sk pk bool b, b \in Name_Red.O_GAKE.sid_pk{2} => oget Name_Red.O_GAKE.sid_pk{2}.[b] = Inner pk bool
-                    => pk \in GAKEb.servers{2} => obind GAKE_mod.get_skey GAKEb.servers{2}.[pk] = Some sk 
+                    => pk \in GAKEb_nodhs.servers{2} => obind GAKE_mod.get_skey GAKEb_nodhs.servers{2}.[pk] = Some sk 
                     => pk = g ^ sk)
 
                /\ (forall pk j x1 x2 x4 x5, pk \notin Name_Red.O_GAKE.pk_set{2} 
-                    => pk \notin GAKE_mod.GAKEb.servers{2} /\ (pk, j) \notin GAKE_mod.GAKEb.s_smap{2} /\ (x1, x2, pk, x4, x5) \notin GAKE_mod.HROc.RO.m{2})
+                    => pk \notin GAKE_mod.GAKEb_nodhs.servers{2} /\ (pk, j) \notin GAKE_mod.GAKEb_nodhs.s_smap{2} /\ (x1, x2, pk, x4, x5) \notin GAKE_mod.HROc.RO.m{2})
 
                /\ (forall b1 b2, b1 \in Name_Red.O_GAKE.sid_pk{2} => b2 \in Name_Red.O_GAKE.sid_pk{2} 
                     => !get_sr_out (oget Name_Red.O_GAKE.sid_pk{2}.[b1]) => !get_sr_out (oget Name_Red.O_GAKE.sid_pk{2}.[b2])  
@@ -1524,7 +1585,6 @@ wp; call (: Name_Red.O_GAKE.stop
 
 - exact A_ll.
 
-admit. (*
 - proc; inline.
   sp 0 1; if {2} => //.
   + if {1} => //.
@@ -1556,13 +1616,14 @@ admit. (*
     if {2} => //.
     + auto => /> &1 &2 *. smt(get_setE mem_set in_fsetU in_fset1).
     auto => /> &1 &2 *. smt(get_setE mem_set in_fsetU in_fset1).
-  auto => /> &1 &2 *.*)
+  auto => /> &1 &2 *.
 - move => &2 bad; proc; inline. auto => />.
   by rewrite weight_dprod dkey_ll dtag_ll //=.
 - move => &1; proc; inline.
   rcondf ^if; auto => />.
 
 - proc; inline.
+  if => //.
   sp; if {2} => //.
   + if => //.
     + auto => />. smt().
@@ -1573,19 +1634,15 @@ admit. (*
     auto => /> &1 &2 *. 
     smt().
   if {1} => //; auto => />.
-- move => &2 bad; proc; inline. if => //; auto => />.
+- move => &2 bad; proc; inline. if => //; sp; if => //; auto => />.
   by rewrite dt_ll bad //=.
 - move => &1; proc; inline.
+  if => //.
   rcondf ^if; auto => />.
 
-- proc; inline.
-  sp 1 1; if {2} => //.
-  + rcondt {1} ^if. auto => /#.
-  + auto => /> &1 &2 *. do !split; smt(get_setE mem_set in_fsetU in_fset1 pow_bij).
-  auto => /> &1 &2 *. smt().
-- move => &2 bad; proc; inline. auto => />.
-- move => &1; proc; inline.
-  rcondf ^if; auto => />.
+- sim />.
+- move => &2 bad; proc; inline; auto => />.
+- move => &1; proc; inline; auto => />.
 
 - proc; inline.
   case (Name_Red.O_GAKE.stop{2}). 
@@ -1722,10 +1779,10 @@ case (1 <= card (get_partners_c t'{1} GAKEb_st.s_smap{1})); 2: smt().
 case (1 <= card (get_untested_partners_c t'{1} GAKEb_st.s_smap{1}) = false); 2: smt().
 move => *.
 right.
-have<-: (card (get_partners_c t'{1} GAKEb_st.s_smap{1}) = card (get_partners_c t'{2} GAKEb.s_smap{2})).
+have<-: (card (get_partners_c t'{1} GAKEb_st.s_smap{1}) = card (get_partners_c t'{2} GAKEb_nodhs.s_smap{2})).
 rewrite /get_partners_c. 
 admit.
-have<-: (card (get_untested_partners_c t'{1} GAKEb_st.s_smap{1}) = card (get_untested_partners_c t'{2} GAKEb.s_smap{2})). admit.
+have<-: (card (get_untested_partners_c t'{1} GAKEb_st.s_smap{1}) = card (get_untested_partners_c t'{2} GAKEb_nodhs.s_smap{2})). admit.
 smt().
  move => [] *. smt(). admit. (* relate untested_partner_c *)
       + auto => />. smt(get_setE mem_set in_fsetU in_fset1 pow_bij).
@@ -1744,10 +1801,10 @@ smt().
       + auto => />.
       move => stl str.
       match {1}. 
-      + match Pending {2} ^match. auto => />.
+      + match Pending {2} ^match. auto => />. admit.
         auto => />.
-      + match Accepted {2} ^match. auto => /#.
-        auto => /> &1 &2 *. split.  move => *. split. rewrite negb_or. split. smt(get_setE mem_set in_fsetU in_fset1 pow_bij). admit. move => *. split.  smt(get_setE mem_set in_fsetU in_fset1 pow_bij). split. 
+      + match Accepted {2} ^match. auto => />. admit.
+        auto => /> &1 &2 *. split.  move => *. split. rewrite negb_or. split. admit. admit. move => *. split. admit. split. 
 move => b1 j1.
 case ((b1, j1) = (b, j){2}) => [[] b1eq j1eq | bjneq].
 rewrite mem_set b1eq j1eq //=.
@@ -1755,7 +1812,7 @@ smt(get_setE mem_set in_fsetU in_fset1 pow_bij).
 rewrite mem_set bjneq //=.
 admit.
 smt(get_setE mem_set in_fsetU in_fset1 pow_bij). admit.
-      match Aborted {2} ^match. auto => /#.
+      match Aborted {2} ^match. auto => />. admit.
       auto => />.
     match None {1} ^match. auto => />. admit. (* A dishonest server is never in s_smap *)
     auto => />.
@@ -1780,7 +1837,9 @@ case (x.`3 = b{2}).
  smt(get_setE mem_set in_fsetU in_fset1 pow_bij).
  smt(get_setE mem_set in_fsetU in_fset1 pow_bij).
 
-split. smt(get_setE mem_set in_fsetU in_fset1 pow_bij). split. 
+split. smt(get_setE mem_set in_fsetU in_fset1 pow_bij). split. smt(get_setE mem_set in_fsetU in_fset1 pow_bij).
+
+split. smt(get_setE mem_set in_fsetU in_fset1 pow_bij). split. smt(get_setE mem_set in_fsetU in_fset1 pow_bij). split. smt(get_setE mem_set in_fsetU in_fset1 pow_bij). split. smt(get_setE mem_set in_fsetU in_fset1 pow_bij). split. smt(get_setE mem_set in_fsetU in_fset1 pow_bij). split. smt(get_setE mem_set in_fsetU in_fset1 pow_bij). split. smt(get_setE mem_set in_fsetU in_fset1 pow_bij). split. smt(get_setE mem_set in_fsetU in_fset1 pow_bij). split. smt(get_setE mem_set in_fsetU in_fset1 pow_bij). split. admit. split. smt(get_setE mem_set in_fsetU in_fset1 pow_bij). split. smt(get_setE mem_set in_fsetU in_fset1 pow_bij). split. smt(get_setE mem_set in_fsetU in_fset1 pow_bij). split. smt(get_setE mem_set in_fsetU in_fset1 pow_bij). split. smt(get_setE mem_set in_fsetU in_fset1 pow_bij).
 move => b1 b2.
 case (b1 = b{2}) => b1eq.
 case (b2 = b{2}) => b2eq. smt(get_setE mem_set in_fsetU in_fset1 pow_bij).
@@ -1789,9 +1848,7 @@ smt(get_setE mem_set in_fsetU in_fset1 pow_bij).
 case (b2 = b{2}) => b2eq. 
 have: get_pkey_mod (oget Name_Red.O_GAKE.sid_pk{2}.[b2]) = pk{2}. smt(get_setE mem_set in_fsetU in_fset1 pow_bij).
 smt(get_setE mem_set in_fsetU in_fset1 pow_bij).
-smt(get_setE mem_set in_fsetU in_fset1 pow_bij).
-
-split. admit. split. smt(get_setE mem_set in_fsetU in_fset1 pow_bij). split. smt(get_setE mem_set in_fsetU in_fset1 pow_bij). split. smt(get_setE mem_set in_fsetU in_fset1 pow_bij). split. smt(get_setE mem_set in_fsetU in_fset1 pow_bij). split. smt(get_setE mem_set in_fsetU in_fset1 pow_bij). split. smt(get_setE mem_set in_fsetU in_fset1 pow_bij). split. admit. split. admit. smt(get_setE mem_set in_fsetU in_fset1 pow_bij). 
+smt(get_setE mem_set in_fsetU in_fset1 pow_bij). 
       auto => />.
     + match Inner {2} ^match. auto => /#.
       match Some {2} ^match. auto => /#.
@@ -1830,11 +1887,11 @@ split. admit. split. smt(get_setE mem_set in_fsetU in_fset1 pow_bij). split. smt
       + auto => />.
       move => stl str.
       match {1}. 
-      + match Pending {2} ^match. auto => /#.
+      + match Pending {2} ^match. auto => />. admit.
         auto => />.
-      + match Accepted {2} ^match. auto => /#.
+      + match Accepted {2} ^match. auto => />. admit.
         auto => /> &1 &2 *. split. move => *. split. admit. move => *. split. admit. split. admit. smt(get_setE mem_set in_fsetU in_fset1 pow_bij). admit.
-      match Aborted {2} ^match. auto => /#.
+      match Aborted {2} ^match. auto => />. admit.
       auto => />.
     match None {1} ^match. auto => />. admit. (* A dishonest server is never in s_smap *)
     auto => />.
@@ -1880,16 +1937,16 @@ split. admit. split. smt(get_setE mem_set in_fsetU in_fset1 pow_bij). split. smt
         + auto => />.
         move => stl str.
         match {1} => //.
-        + match Pending {2} ^match. auto => /#.
+        + match Pending {2} ^match. auto => />. admit.
           auto => />.
-        + match Accepted {2} ^match. auto => /#.
+        + match Accepted {2} ^match. auto => />. admit.
           if => //.
           + auto => &1 &2 *. admit.
           + if => //.
-            + auto => /> &1 &2 *. split. smt(get_setE mem_set in_fsetU in_fset1). split. admit. admit.
+            + auto => /> &1 &2 *. split. admit. split. admit. admit.
             auto => /> &1 &2 *. split. admit. admit.
           auto => />.
-        match Aborted {2} ^match. auto => /#.
+        match Aborted {2} ^match. auto => />. admit.
         auto => />.
       auto => />.
     if {1} => //.
@@ -1906,6 +1963,6 @@ split. admit. split. smt(get_setE mem_set in_fsetU in_fset1 pow_bij). split. smt
 
 auto => />.
 split. smt(emptyE in_fset0).
-move => roeq inj csm ssm pkin inv inv2 inv3 inv4 inv5 inv6 inv7 inv8 inv9 inv10 inv11 inv12 inv13 inv14 inv15 rl rr al csl pksl ssl sl stl tl url ml ar csr tr str huh ssr sr pksr urr mr.
+move => roeq inj csm ssm pkin inv inv2 inv3 inv4 inv5 inv6 inv7 inv8 inv9 inv10 inv11 inv12 inv13 inv14 inv15 inv16 inv17 inv18 inv19 inv20 inv21 rl rr al hsl csl pksl ssl sl stl tl url ml ar hsr csr tr str huh ssr sr pksr urr mr.
 by case : (!str) => />.
 qed.
